steel/formats/steel/Zeta.Steel.LogEntry.fst
@@ -31,7 +31,18 @@ let parse32_log_entry
 let parser_log_entry =
   Zeta.Steel.FormatsLib.mk_steel_parser parse32_log_entry
 
-let runapp_payload_offset e =
+let runapp_payload_offset'
+  (e: log_entry)
+: Pure U32.t
+  (requires (RunApp? e))
+  (ensures (fun res ->
+    let s = Zeta.Formats.LogEntry.serialize_log_entry e in
+    let RunApp r = e in
+    let off = U32.v res in
+    off <= Seq.length s /\
+    Ghost.reveal r.rest.ebytes `Seq.equal` Seq.slice s off (Seq.length s)
+  ))
+=
   let RunApp r = e in
   let b = Ghost.hide (FStar.Bytes.hide (Ghost.reveal r.rest.ebytes)) in
   let h = synth_log_entry_recip_hdr e in
@@ -46,13 +57,14 @@ let runapp_payload_offset e =
     (Ghost.reveal b)
   ;
   assert (LowParse.Spec.Bytes.serialize_bounded_vlbytes 0 2147483647 (Ghost.reveal b) == LowParse.Spec.VLData.serialize_bounded_integer 4 r.rest.len `Seq.append` r.rest.ebytes);
-  let res =
-    Zeta.Formats.Aux.Log_entry_hdr.log_entry_hdr_size32 h `U32.add` 4ul
-  in
-  assert (
-    let s = spec_serializer_log_entry e in
-    let off = U32.v res in
-    off <= Seq.length s /\
-    Ghost.reveal r.rest.ebytes `Seq.equal` Seq.slice s off (Seq.length s)
-  );
-  res
+  Zeta.Formats.Aux.Log_entry_hdr.log_entry_hdr_size32 h `U32.add` 4ul
+
+#push-options "--z3rlimit 32"
+
+let runapp_payload_offset
+  e b
+=
+  LowParse.Spec.Base.parse_injective Zeta.Formats.LogEntry.parse_log_entry b (Zeta.Formats.LogEntry.serialize_log_entry e);
+  runapp_payload_offset' e
+
+#pop-options
